Added some missing protobuf types

protobuf-shim/src/lib.rs
@@ -1,4 +1,4 @@
-mod enums {
+pub mod enums {
     use core::fmt;
     /// Trait implemented by all protobuf enum types.
     ///
@@ -26,5 +26,117 @@ mod enums {
 
         /// All enum values for enum type.
         const VALUES: &'static [Self];
+    }
+}
+
+pub mod special {
+    pub struct SpecialFields {
+        unknown_fields: crate::unknown_fields::UnknownFields,
+        cached_size: crate::cached_size::CachedSize,
+    }   
+}
+
+pub mod cached_size {
+    /// Cached size field used in generated code.
+    ///
+    /// It is always equal to itself to simplify generated code.
+    /// (Generated code can use `#[derive(Eq)]`).
+    ///
+    /// This type should rarely be used directly.
+    #[derive(Debug, Default)]
+    pub struct CachedSize {
+        size: (),
+    }
+}
+
+pub mod unknown_fields {
+
+    /// Hold "unknown" fields in parsed message.
+    ///
+    /// Field may be unknown if it they are added in newer version of `.proto`.
+    /// Unknown fields are stored in `UnknownFields` structure, so
+    /// protobuf message could process messages without losing data.
+    ///
+    /// For example, in this operation: load from DB, modify, store to DB,
+    /// even when working with older `.proto` file, new fields won't be lost.
+    #[derive(Clone, PartialEq, Eq, Debug, Default)]
+    pub struct UnknownFields {
+        /// The map.
+        //
+        // `Option` is needed, because HashMap constructor performs allocation,
+        // and very expensive.
+        //
+        // We use "default hasher" to make iteration order deterministic.
+        // Which is used to make codegen output deterministic in presence of unknown fields
+        // (e. g. file options are represented as unknown fields).
+        // Using default hasher is suboptimal, because it makes unknown fields less safe.
+        // Note, Google Protobuf C++ simply uses linear map (which can exploitable the same way),
+        // and Google Protobuf Java uses tree map to store unknown fields
+        // (which is more expensive than hashmap).
+        fields: (),
+    }
+}
+
+pub mod message_field {
+    pub struct MessageField<T>(pub Option<Box<T>>);
+}
+
+pub mod enum_or_unknown {
+    pub struct EnumOrUnknown<E> {
+        phantom: std::marker::PhantomData<E>,
+    }
+}
+
+pub mod oneof {
+    pub trait Oneof {}
+}
+
+
+pub mod oneof_full {
+    use crate::oneof::Oneof;
+    use crate::reflect::OneofDescriptor;
+
+    /// Implemented by all oneof types when lite runtime is not enabled.
+    pub trait OneofFull: Oneof { 
+        /// Descriptor object for this oneof.
+        fn descriptor() -> OneofDescriptor;
+    }
+}
+
+pub mod reflect {
+    pub struct OneofDescriptor {
+        _hax_placeholder: (),
+    }
+
+    pub struct EnumValueDescriptor {
+        _hax_placeholder: (),
+    }
+
+    pub struct EnumDescriptor {
+        _hax_placeholder: (),
+    }
+}
+
+pub mod marker {
+    pub trait Copy: Clone {}
+
+    pub trait Clone: Sized {
+        // Required method
+        fn clone(&self) -> Self;
+
+        fn clone_from(&mut self, source: &Self) {
+            *self = source.clone()
+        }
+    }
+}
+
+pub mod enum_full {
+    use crate::enums::*;
+    use crate::reflect::*;
+
+    pub trait EnumFull: Enum {
+        // Required methods
+        fn descriptor(&self) -> EnumValueDescriptor;
+        fn enum_descriptor() -> EnumDescriptor;
     }
 }
