rust_vendor/sandwich-proto/proofs/fstar/extraction/Sandwich_proto.Errors.fsti
@@ -3,14 +3,223 @@ module Sandwich_proto.Errors
 open Core
 open FStar.Mul
 
+let _ =
+  (* This module has implicit dependencies, here we make them explicit. *)
+  (* The implicit dependencies arise from typeclasses instances. *)
+  let open Protobuf.Enums in
+  ()
+
+type t_ALPNError =
+  | ALPNError_ALPNERROR_LENGTH_ERROR : t_ALPNError
+  | ALPNError_ALPNERROR_INVALID_STRING : t_ALPNError
+
+[@@ FStar.Tactics.Typeclasses.tcinstance]
+val impl_30:Core.Default.t_Default t_ALPNError
+
+[@@ FStar.Tactics.Typeclasses.tcinstance]
+val impl_28:Protobuf.Enums.t_Enum t_ALPNError
+
+[@@ FStar.Tactics.Typeclasses.tcinstance]
+val impl_29:Protobuf.Enum_full.t_EnumFull t_ALPNError
+
+type t_APIError =
+  | APIError_APIERROR_CONFIGURATION : t_APIError
+  | APIError_APIERROR_SOCKET : t_APIError
+  | APIError_APIERROR_TUNNEL : t_APIError
+
+[@@ FStar.Tactics.Typeclasses.tcinstance]
+val impl_2:Core.Default.t_Default t_APIError
+
+[@@ FStar.Tactics.Typeclasses.tcinstance]
+val impl:Protobuf.Enums.t_Enum t_APIError
+
+[@@ FStar.Tactics.Typeclasses.tcinstance]
+val impl_1:Protobuf.Enum_full.t_EnumFull t_APIError
+
 type t_ASN1Error =
   | ASN1Error_ASN1ERROR_INVALID_FORMAT : t_ASN1Error
   | ASN1Error_ASN1ERROR_MALFORMED : t_ASN1Error
+
+[@@ FStar.Tactics.Typeclasses.tcinstance]
+val impl_26:Core.Default.t_Default t_ASN1Error
+
+[@@ FStar.Tactics.Typeclasses.tcinstance]
+val impl_24:Protobuf.Enums.t_Enum t_ASN1Error
+
+[@@ FStar.Tactics.Typeclasses.tcinstance]
+val impl_25:Protobuf.Enum_full.t_EnumFull t_ASN1Error
+
+type t_CertificateError =
+  | CertificateError_CERTIFICATEERROR_MALFORMED : t_CertificateError
+  | CertificateError_CERTIFICATEERROR_EXPIRED : t_CertificateError
+  | CertificateError_CERTIFICATEERROR_NOT_FOUND : t_CertificateError
+  | CertificateError_CERTIFICATEERROR_UNKNOWN : t_CertificateError
+  | CertificateError_CERTIFICATEERROR_UNSUPPORTED : t_CertificateError
+
+[@@ FStar.Tactics.Typeclasses.tcinstance]
+val impl_18:Core.Default.t_Default t_CertificateError
+
+[@@ FStar.Tactics.Typeclasses.tcinstance]
+val impl_16:Protobuf.Enums.t_Enum t_CertificateError
+
+[@@ FStar.Tactics.Typeclasses.tcinstance]
+val impl_17:Protobuf.Enum_full.t_EnumFull t_CertificateError
+
+type t_ConfigurationError =
+  | ConfigurationError_CONFIGURATIONERROR_INVALID_IMPLEMENTATION : t_ConfigurationError
+  | ConfigurationError_CONFIGURATIONERROR_UNSUPPORTED_IMPLEMENTATION : t_ConfigurationError
+  | ConfigurationError_CONFIGURATIONERROR_INVALID : t_ConfigurationError
+  | ConfigurationError_CONFIGURATIONERROR_INVALID_LISTENER : t_ConfigurationError
+
+[@@ FStar.Tactics.Typeclasses.tcinstance]
+val impl_6:Core.Default.t_Default t_ConfigurationError
+
+[@@ FStar.Tactics.Typeclasses.tcinstance]
+val impl_4:Protobuf.Enums.t_Enum t_ConfigurationError
+
+[@@ FStar.Tactics.Typeclasses.tcinstance]
+val impl_5:Protobuf.Enum_full.t_EnumFull t_ConfigurationError
 
 type t_DataSourceError =
   | DataSourceError_DATASOURCEERROR_EMPTY : t_DataSourceError
   | DataSourceError_DATASOURCEERROR_INVALID_CASE : t_DataSourceError
   | DataSourceError_DATASOURCEERROR_NOT_FOUND : t_DataSourceError
+
+[@@ FStar.Tactics.Typeclasses.tcinstance]
+val impl_34:Core.Default.t_Default t_DataSourceError
+
+[@@ FStar.Tactics.Typeclasses.tcinstance]
+val impl_32:Protobuf.Enums.t_Enum t_DataSourceError
+
+[@@ FStar.Tactics.Typeclasses.tcinstance]
+val impl_33:Protobuf.Enum_full.t_EnumFull t_DataSourceError
+
+type t_ErrorKind =
+  | ErrorKind_ERRORKIND_API : t_ErrorKind
+  | ErrorKind_ERRORKIND_CONFIGURATION : t_ErrorKind
+  | ErrorKind_ERRORKIND_TLS_CONFIGURATION : t_ErrorKind
+  | ErrorKind_ERRORKIND_CERTIFICATE : t_ErrorKind
+  | ErrorKind_ERRORKIND_SYSTEM : t_ErrorKind
+  | ErrorKind_ERRORKIND_SOCKET : t_ErrorKind
+  | ErrorKind_ERRORKIND_PROTOBUF : t_ErrorKind
+  | ErrorKind_ERRORKIND_PRIVATE_KEY : t_ErrorKind
+  | ErrorKind_ERRORKIND_ASN1 : t_ErrorKind
+  | ErrorKind_ERRORKIND_DATA_SOURCE : t_ErrorKind
+  | ErrorKind_ERRORKIND_KEM : t_ErrorKind
+  | ErrorKind_ERRORKIND_HANDSHAKE : t_ErrorKind
+  | ErrorKind_ERRORKIND_TUNNEL : t_ErrorKind
+  | ErrorKind_ERRORKIND_ALPN : t_ErrorKind
+  | ErrorKind_ERRORKIND_IO : t_ErrorKind
+
+[@@ FStar.Tactics.Typeclasses.tcinstance]
+val impl_58:Core.Default.t_Default t_ErrorKind
+
+[@@ FStar.Tactics.Typeclasses.tcinstance]
+val impl_56:Protobuf.Enums.t_Enum t_ErrorKind
+
+[@@ FStar.Tactics.Typeclasses.tcinstance]
+val impl_57:Protobuf.Enum_full.t_EnumFull t_ErrorKind
+
+type t_HandshakeError =
+  | HandshakeError_HANDSHAKEERROR_INVALID_SERVER_NAME : t_HandshakeError
+  | HandshakeError_HANDSHAKEERROR_CERTIFICATE_VERIFICATION_FAILED : t_HandshakeError
+  | HandshakeError_HANDSHAKEERROR_CERTIFICATE_EXPIRED : t_HandshakeError
+  | HandshakeError_HANDSHAKEERROR_CERTIFICATE_REVOKED : t_HandshakeError
+  | HandshakeError_HANDSHAKEERROR_INVALID_CERTIFICATE : t_HandshakeError
+  | HandshakeError_HANDSHAKEERROR_CERTIFICATE_SIGNATURE_VERIFICATION_FAILED : t_HandshakeError
+  | HandshakeError_HANDSHAKEERROR_DEPTH_EXCEEDED : t_HandshakeError
+  | HandshakeError_HANDSHAKEERROR_UNSUPPORTED_PROTOCOL : t_HandshakeError
+  | HandshakeError_HANDSHAKEERROR_NO_SHARED_CIPHER : t_HandshakeError
+  | HandshakeError_HANDSHAKEERROR_NO_SUITABLE_KEY_SHARE : t_HandshakeError
+  | HandshakeError_HANDSHAKEERROR_UNKNOWN_ERROR : t_HandshakeError
+
+[@@ FStar.Tactics.Typeclasses.tcinstance]
+val impl_50:Core.Default.t_Default t_HandshakeError
+
+[@@ FStar.Tactics.Typeclasses.tcinstance]
+val impl_48:Protobuf.Enums.t_Enum t_HandshakeError
+
+[@@ FStar.Tactics.Typeclasses.tcinstance]
+val impl_49:Protobuf.Enum_full.t_EnumFull t_HandshakeError
+
+type t_KEMError =
+  | KEMError_KEMERROR_INVALID : t_KEMError
+  | KEMError_KEMERROR_TOO_MANY : t_KEMError
+
+[@@ FStar.Tactics.Typeclasses.tcinstance]
+val impl_38:Core.Default.t_Default t_KEMError
+
+[@@ FStar.Tactics.Typeclasses.tcinstance]
+val impl_36:Protobuf.Enums.t_Enum t_KEMError
+
+[@@ FStar.Tactics.Typeclasses.tcinstance]
+val impl_37:Protobuf.Enum_full.t_EnumFull t_KEMError
+
+type t_PrivateKeyError =
+  | PrivateKeyError_PRIVATEKEYERROR_MALFORMED : t_PrivateKeyError
+  | PrivateKeyError_PRIVATEKEYERROR_NOT_FOUND : t_PrivateKeyError
+  | PrivateKeyError_PRIVATEKEYERROR_UNKNOWN : t_PrivateKeyError
+  | PrivateKeyError_PRIVATEKEYERROR_UNSUPPORTED : t_PrivateKeyError
+  | PrivateKeyError_PRIVATEKEYERROR_NOT_SERVER : t_PrivateKeyError
+
+[@@ FStar.Tactics.Typeclasses.tcinstance]
+val impl_22:Core.Default.t_Default t_PrivateKeyError
+
+[@@ FStar.Tactics.Typeclasses.tcinstance]
+val impl_20:Protobuf.Enums.t_Enum t_PrivateKeyError
+
+[@@ FStar.Tactics.Typeclasses.tcinstance]
+val impl_21:Protobuf.Enum_full.t_EnumFull t_PrivateKeyError
+
+type t_ProtobufError =
+  | ProtobufError_PROTOBUFERROR_EMPTY : t_ProtobufError
+  | ProtobufError_PROTOBUFERROR_TOO_BIG : t_ProtobufError
+  | ProtobufError_PROTOBUFERROR_PARSE_FAILED : t_ProtobufError
+  | ProtobufError_PROTOBUFERROR_NULLPTR : t_ProtobufError
+  | ProtobufError_PROTOBUFERROR_INVALID_ARGUMENT : t_ProtobufError
+
+[@@ FStar.Tactics.Typeclasses.tcinstance]
+val impl_10:Core.Default.t_Default t_ProtobufError
+
+[@@ FStar.Tactics.Typeclasses.tcinstance]
+val impl_8:Protobuf.Enums.t_Enum t_ProtobufError
+
+[@@ FStar.Tactics.Typeclasses.tcinstance]
+val impl_9:Protobuf.Enum_full.t_EnumFull t_ProtobufError
+
+type t_SocketError =
+  | SocketError_SOCKETERROR_BAD_FD : t_SocketError
+  | SocketError_SOCKETERROR_CREATION_FAILED : t_SocketError
+  | SocketError_SOCKETERROR_BAD_NETADDR : t_SocketError
+  | SocketError_SOCKETERROR_NETADDR_UNKNOWN : t_SocketError
+  | SocketError_SOCKETERROR_FSTAT_FAILED : t_SocketError
+  | SocketError_SOCKETERROR_NOT_SOCK : t_SocketError
+  | SocketError_SOCKETERROR_GETSOCKNAME_FAILED : t_SocketError
+  | SocketError_SOCKETERROR_SETSOCKOPT_FAILED : t_SocketError
+  | SocketError_SOCKETERROR_INVALID_AI_FAMILY : t_SocketError
+
+[@@ FStar.Tactics.Typeclasses.tcinstance]
+val impl_46:Core.Default.t_Default t_SocketError
+
+[@@ FStar.Tactics.Typeclasses.tcinstance]
+val impl_44:Protobuf.Enums.t_Enum t_SocketError
+
+[@@ FStar.Tactics.Typeclasses.tcinstance]
+val impl_45:Protobuf.Enum_full.t_EnumFull t_SocketError
+
+type t_SystemError =
+  | SystemError_SYSTEMERROR_MEMORY : t_SystemError
+  | SystemError_SYSTEMERROR_INTEGER_OVERFLOW : t_SystemError
+  | SystemError_SYSTEMERROR_BACKEND : t_SystemError
+
+[@@ FStar.Tactics.Typeclasses.tcinstance]
+val impl_42:Core.Default.t_Default t_SystemError
+
+[@@ FStar.Tactics.Typeclasses.tcinstance]
+val impl_40:Protobuf.Enums.t_Enum t_SystemError
+
+[@@ FStar.Tactics.Typeclasses.tcinstance]
+val impl_41:Protobuf.Enum_full.t_EnumFull t_SystemError
 
 type t_TLSConfigurationError =
   | TLSConfigurationError_TLSCONFIGURATIONERROR_UNSUPPORTED_IMPLEMENTATION : t_TLSConfigurationError
@@ -22,7 +231,25 @@ type t_TLSConfigurationError =
   | TLSConfigurationError_TLSCONFIGURATIONERROR_UNSUPPORTED_CONTROL_CHARACTERS : t_TLSConfigurationError
   | TLSConfigurationError_TLSCONFIGURATIONERROR_INVALID : t_TLSConfigurationError
 
+[@@ FStar.Tactics.Typeclasses.tcinstance]
+val impl_14:Core.Default.t_Default t_TLSConfigurationError
+
+[@@ FStar.Tactics.Typeclasses.tcinstance]
+val impl_12:Protobuf.Enums.t_Enum t_TLSConfigurationError
+
+[@@ FStar.Tactics.Typeclasses.tcinstance]
+val impl_13:Protobuf.Enum_full.t_EnumFull t_TLSConfigurationError
+
 type t_TunnelError =
   | TunnelError_TUNNELERROR_INVALID : t_TunnelError
   | TunnelError_TUNNELERROR_VERIFIER : t_TunnelError
   | TunnelError_TUNNELERROR_UNKNOWN : t_TunnelError
+
+[@@ FStar.Tactics.Typeclasses.tcinstance]
+val impl_54:Core.Default.t_Default t_TunnelError
+
+[@@ FStar.Tactics.Typeclasses.tcinstance]
+val impl_52:Protobuf.Enums.t_Enum t_TunnelError
+
+[@@ FStar.Tactics.Typeclasses.tcinstance]
+val impl_53:Protobuf.Enum_full.t_EnumFull t_TunnelError
