protobuf-shim/proofs/fstar/extraction/Protobuf.Cached_size.fsti
@@ -1,0 +1,10 @@
+module Protobuf.Cached_size
+#set-options "--fuel 0 --ifuel 1 --z3rlimit 15"
+open Core
+open FStar.Mul
+
+/// Cached size field used in generated code.
+/// It is always equal to itself to simplify generated code.
+/// (Generated code can use `#[derive(Eq)]`).
+/// This type should rarely be used directly.
+type t_CachedSize = { f_size:Prims.unit }
