protobuf-shim/proofs/fstar/extraction/Protobuf.Enum_full.fsti
@@ -1,0 +1,26 @@
+module Protobuf.Enum_full
+#set-options "--fuel 0 --ifuel 1 --z3rlimit 15"
+open Core
+open FStar.Mul
+
+let _ =
+  (* This module has implicit dependencies, here we make them explicit. *)
+  (* The implicit dependencies arise from typeclasses instances. *)
+  let open Protobuf.Enums in
+  ()
+
+class t_EnumFull (#v_Self: Type0) = {
+  [@@@ FStar.Tactics.Typeclasses.no_method]_super_14911585333008767414:Protobuf.Enums.t_Enum #v_Self;
+  f_descriptor_pre:v_Self -> bool;
+  f_descriptor_post:v_Self -> Protobuf.Reflect.t_EnumValueDescriptor -> bool;
+  f_descriptor:x0: v_Self
+    -> Prims.Pure Protobuf.Reflect.t_EnumValueDescriptor
+        (f_descriptor_pre x0)
+        (fun result -> f_descriptor_post x0 result);
+  f_enum_descriptor_pre:Prims.unit -> bool;
+  f_enum_descriptor_post:Prims.unit -> Protobuf.Reflect.t_EnumDescriptor -> bool;
+  f_enum_descriptor:x0: Prims.unit
+    -> Prims.Pure Protobuf.Reflect.t_EnumDescriptor
+        (f_enum_descriptor_pre x0)
+        (fun result -> f_enum_descriptor_post x0 result)
+}
