protobuf-shim/proofs/fstar/extraction/Protobuf.Enum_or_unknown.fsti
@@ -1,0 +1,6 @@
+module Protobuf.Enum_or_unknown
+#set-options "--fuel 0 --ifuel 1 --z3rlimit 15"
+open Core
+open FStar.Mul
+
+type t_EnumOrUnknown (v_E: Type0) = { f_phantom:Core.Marker.t_PhantomData v_E }
