protobuf-shim/proofs/fstar/extraction/Protobuf.Marker.fsti
@@ -1,0 +1,18 @@
+module Protobuf.Marker
+#set-options "--fuel 0 --ifuel 1 --z3rlimit 15"
+open Core
+open FStar.Mul
+
+class t_Clone (v_Self: Type0) = {
+  f_clone_pre:v_Self -> bool;
+  f_clone_post:v_Self -> v_Self -> bool;
+  f_clone:x0: v_Self -> Prims.Pure v_Self (f_clone_pre x0) (fun result -> f_clone_post x0 result);
+  f_clone_from_pre:v_Self -> v_Self -> bool;
+  f_clone_from_post:v_Self -> v_Self -> v_Self -> bool;
+  f_clone_from:x0: v_Self -> x1: v_Self
+    -> Prims.Pure v_Self (f_clone_from_pre x0 x1) (fun result -> f_clone_from_post x0 x1 result)
+}
+
+class t_Copy (v_Self: Type0) = {
+  [@@@ FStar.Tactics.Typeclasses.no_method]_super_13225068822189715818:t_Clone v_Self
+}
