protobuf-shim/proofs/fstar/extraction/Protobuf.Message_field.fsti
@@ -1,0 +1,8 @@
+module Protobuf.Message_field
+#set-options "--fuel 0 --ifuel 1 --z3rlimit 15"
+open Core
+open FStar.Mul
+
+type t_MessageField (v_T: Type0) =
+  | MessageField : Core.Option.t_Option (Alloc.Boxed.t_Box v_T Alloc.Alloc.t_Global)
+    -> t_MessageField v_T
