protobuf-shim/proofs/fstar/extraction/Protobuf.Oneof.fsti
@@ -1,0 +1,6 @@
+module Protobuf.Oneof
+#set-options "--fuel 0 --ifuel 1 --z3rlimit 15"
+open Core
+open FStar.Mul
+
+class t_Oneof (#v_Self: Type0) = { __marker_trait_t_Oneof:Prims.unit }
