protobuf-shim/proofs/fstar/extraction/Protobuf.Reflect.fsti
@@ -1,0 +1,10 @@
+module Protobuf.Reflect
+#set-options "--fuel 0 --ifuel 1 --z3rlimit 15"
+open Core
+open FStar.Mul
+
+type t_EnumDescriptor = { f_hax_placeholder:Prims.unit }
+
+type t_EnumValueDescriptor = { f_hax_placeholder:Prims.unit }
+
+type t_OneofDescriptor = { f_hax_placeholder:Prims.unit }
