protobuf-shim/proofs/fstar/extraction/Protobuf.Special.fsti
@@ -1,0 +1,9 @@
+module Protobuf.Special
+#set-options "--fuel 0 --ifuel 1 --z3rlimit 15"
+open Core
+open FStar.Mul
+
+type t_SpecialFields = {
+  f_unknown_fields:Protobuf.Unknown_fields.t_UnknownFields;
+  f_cached_size:Protobuf.Cached_size.t_CachedSize
+}
