protobuf-shim/proofs/fstar/extraction/Protobuf.Unknown_fields.fsti
@@ -1,0 +1,12 @@
+module Protobuf.Unknown_fields
+#set-options "--fuel 0 --ifuel 1 --z3rlimit 15"
+open Core
+open FStar.Mul
+
+/// Hold "unknown" fields in parsed message.
+/// Field may be unknown if it they are added in newer version of `.proto`.
+/// Unknown fields are stored in `UnknownFields` structure, so
+/// protobuf message could process messages without losing data.
+/// For example, in this operation: load from DB, modify, store to DB,
+/// even when working with older `.proto` file, new fields won't be lost.
+type t_UnknownFields = { f_fields:Prims.unit }
