rust_vendor/sandwich-api-proto/proofs/fstar/extraction/Protobuf.Message_full.fsti
@@ -1,0 +1,6 @@
+module Protobuf.Message_full
+open Core
+
+class t_MessageFull (#v_Self : Type0) = {
+    dummy_field : unit
+}
