rust_vendor/sandwich-api-proto/proofs/fstar/extraction/Sandwich_api_proto.Compliance.fsti
@@ -6,10 +6,10 @@ open FStar.Mul
 let _ =
   (* This module has implicit dependencies, here we make them explicit. *)
   (* The implicit dependencies arise from typeclasses instances. *)
-  // let open Protobuf.Enums in
-  // let open Protobuf.Message in
-  // let open Protobuf.Reflect.Runtime_types in
-  // let open Protobuf.Reflect.Value in
+  let open Protobuf.Enums in
+  let open Protobuf.Message in
+  let open Protobuf.Reflect.Runtime_types in
+  let open Protobuf.Reflect.Value in
   ()
 
 type t_ClassicalAlgoChoice =
@@ -17,26 +17,26 @@ type t_ClassicalAlgoChoice =
   | ClassicalAlgoChoice_CLASSICAL_ALGORITHMS_FORBID : t_ClassicalAlgoChoice
 
 [@@ FStar.Tactics.Typeclasses.tcinstance]
-val impl_8:Core.Default.t_Default #t_ClassicalAlgoChoice
+val impl_8:Core.Default.t_Default t_ClassicalAlgoChoice
 
 [@@ FStar.Tactics.Typeclasses.tcinstance]
-val impl_6:Protobuf.Enums.t_Enum #t_ClassicalAlgoChoice
+val impl_6:Protobuf.Enums.t_Enum t_ClassicalAlgoChoice
 
 [@@ FStar.Tactics.Typeclasses.tcinstance]
-val impl_7:Protobuf.Enum_full.t_EnumFull #t_ClassicalAlgoChoice
+val impl_7:Protobuf.Enum_full.t_EnumFull t_ClassicalAlgoChoice
 
 type t_HybridAlgoChoice =
   | HybridAlgoChoice_HYBRID_ALGORITHMS_ALLOW : t_HybridAlgoChoice
   | HybridAlgoChoice_HYBRID_ALGORITHMS_FORBID : t_HybridAlgoChoice
 
 [@@ FStar.Tactics.Typeclasses.tcinstance]
-val impl_16:Core.Default.t_Default #t_HybridAlgoChoice
+val impl_16:Core.Default.t_Default t_HybridAlgoChoice
 
 [@@ FStar.Tactics.Typeclasses.tcinstance]
-val impl_14:Protobuf.Enums.t_Enum #t_HybridAlgoChoice
+val impl_14:Protobuf.Enums.t_Enum t_HybridAlgoChoice
 
 [@@ FStar.Tactics.Typeclasses.tcinstance]
-val impl_15:Protobuf.Enum_full.t_EnumFull #t_HybridAlgoChoice
+val impl_15:Protobuf.Enum_full.t_EnumFull t_HybridAlgoChoice
 
 type t_NISTSecurityStrengthBits =
   | NISTSecurityStrengthBits_BIT_STRENGTH_AT_LEAST_128_ : t_NISTSecurityStrengthBits
@@ -44,26 +44,26 @@ type t_NISTSecurityStrengthBits =
   | NISTSecurityStrengthBits_BIT_STRENGTH_AT_LEAST_256_ : t_NISTSecurityStrengthBits
 
 [@@ FStar.Tactics.Typeclasses.tcinstance]
-val impl_20:Core.Default.t_Default #t_NISTSecurityStrengthBits
+val impl_20:Core.Default.t_Default t_NISTSecurityStrengthBits
 
 [@@ FStar.Tactics.Typeclasses.tcinstance]
-val impl_18:Protobuf.Enums.t_Enum #t_NISTSecurityStrengthBits
+val impl_18:Protobuf.Enums.t_Enum t_NISTSecurityStrengthBits
 
 [@@ FStar.Tactics.Typeclasses.tcinstance]
-val impl_19:Protobuf.Enum_full.t_EnumFull #t_NISTSecurityStrengthBits
+val impl_19:Protobuf.Enum_full.t_EnumFull t_NISTSecurityStrengthBits
 
 type t_QuantumSafeAlgoChoice =
   | QuantumSafeAlgoChoice_QUANTUM_SAFE_ALGORITHMS_ALLOW : t_QuantumSafeAlgoChoice
   | QuantumSafeAlgoChoice_QUANTUM_SAFE_ALGORITHMS_FORBID : t_QuantumSafeAlgoChoice
 
 [@@ FStar.Tactics.Typeclasses.tcinstance]
-val impl_12:Core.Default.t_Default #t_QuantumSafeAlgoChoice
+val impl_12:Core.Default.t_Default t_QuantumSafeAlgoChoice
 
 [@@ FStar.Tactics.Typeclasses.tcinstance]
-val impl_10:Protobuf.Enums.t_Enum #t_QuantumSafeAlgoChoice
+val impl_10:Protobuf.Enums.t_Enum t_QuantumSafeAlgoChoice
 
 [@@ FStar.Tactics.Typeclasses.tcinstance]
-val impl_11:Protobuf.Enum_full.t_EnumFull #t_QuantumSafeAlgoChoice
+val impl_11:Protobuf.Enum_full.t_EnumFull t_QuantumSafeAlgoChoice
 
 type t_Compliance = {
   f_hybrid_choice:Protobuf.Enum_or_unknown.t_EnumOrUnknown t_HybridAlgoChoice;
@@ -74,16 +74,16 @@ type t_Compliance = {
 }
 
 [@@ FStar.Tactics.Typeclasses.tcinstance]
-val impl:Core.Default.t_Default #t_Compliance
+val impl:Core.Default.t_Default t_Compliance
 
 [@@ FStar.Tactics.Typeclasses.tcinstance]
-val impl_2:Protobuf.Message.t_Message #t_Compliance
+val impl_2:Protobuf.Message.t_Message t_Compliance
 
 [@@ FStar.Tactics.Typeclasses.tcinstance]
-val impl_4:Core.Fmt.t_Display #t_Compliance
+val impl_4:Core.Fmt.t_Display t_Compliance
 
 [@@ FStar.Tactics.Typeclasses.tcinstance]
-val impl_3:Protobuf.Message_full.t_MessageFull #t_Compliance
+val impl_3:Protobuf.Message_full.t_MessageFull t_Compliance
 
 [@@ FStar.Tactics.Typeclasses.tcinstance]
-val impl_5:Protobuf.Reflect.Value.t_ProtobufValue #t_Compliance
+val impl_5:Protobuf.Reflect.Value.t_ProtobufValue t_Compliance
