rust_vendor/sandwich-api-proto/proofs/fstar/extraction/Sandwich_api_proto.Data_source.Data_source.fsti
@@ -1,0 +1,9 @@
+module Sandwich_api_proto.Data_source.Data_source
+#set-options "--fuel 0 --ifuel 1 --z3rlimit 15"
+open Core
+open FStar.Mul
+
+type t_Specifier =
+  | Specifier_Filename : Alloc.String.t_String -> t_Specifier
+  | Specifier_InlineBytes : Alloc.Vec.t_Vec u8 Alloc.Alloc.t_Global -> t_Specifier
+  | Specifier_InlineString : Alloc.String.t_String -> t_Specifier
